BasicRules.v
@@ -5,6 +5,8 @@ Require Import Toy.type.
 Require Import Toy.UnifySL.implementation.
 Require Import Toy.Language.
 Require Import Toy.Embeddings.
+Require Import Coq.micromega.Psatz.
+Require Import Lqa.
 Open Scope Z.
 Import T.
 Import Denote_Aexp Denote_Bexp Denote_Term Denote_Assertion_D Denote_Com.
@@ -153,7 +155,7 @@ Proof.
   simpl; tauto.
 Qed.
 
-Lemma andjoin : forall e v st1 st2 st,
+Lemma andjoin1 : forall e v st1 st2 st,
   aeval e st1 = Some v ->
   stateJ st1 st2 st ->
   aeval e st = Some v.
@@ -203,29 +205,212 @@ Proof.
     rewrite H4 in H.
     ufHeapj H1.
     specialize (H1 p).
-    Print ufoptionj.
-    pose proof (ufoptionj _ (snd st1 p)).
-    rewrite ufoptionj in H1.
-
- 
-  
-  
-  
-  admit.
-Admitted.
-
+    pose proof (ufoptionj QZandLock_Join (snd st1 p) (snd st2 p) (snd st p)).
+    rewrite H5 in H1; clear H5.
+    destruct H1 as [? | [? | [? | ?]]].
+    - destruct H1 as [? [? ?]]. rewrite H4 in H1; inversion H1.
+    - destruct H1 as [x' [? [? ?]]]. rewrite H4 in H1; inversion H1.
+    - destruct H1 as [x' [? [? ?]]]. 
+      rewrite H4 in H1; inversion H1; subst x'.
+      rewrite H6, H. tauto.
+    - rename x into x1.
+      destruct H1 as [x1' [x2 [x [? [? [? ?]]]]]].
+      rewrite H4 in H1; inversion H1; subst x1'. rewrite H6.
+      unfold QZandLock_Join in H7.
+      rewrite ufsumj in H7. destruct H7.
+      2:{ destruct H7 as [xr1 [xr2 [xr [? [? [? ?]]]]]].
+        rewrite H7 in H. inversion H. }
+      destruct H7 as [xr1 [xr2 [xr [? [? [? ?]]]]]].
+      rewrite H7 in H. rewrite H9.
+      unfold QZ_Join in H10.
+      unfold OSAGenerators.prod_Join in H10.
+      destruct H10.
+      unfold SeparationAlgebra.join in H11.
+      unfold Z_Join in H11.
+      unfold OSAGenerators.equiv_Join in H11.
+      destruct H11.
+      destruct xr1 as (q1, v1).
+      destruct xr as (q0, v0).
+      unfold snd in H11. rewrite <-H11.
+      unfold SeparationAlgebra.join in H10.
+      unfold Q_Join in H10. unfold fst in H10.
+      destruct (Qlt_le_dec 0 q1). 2:{ lra. }
+      destruct (Qlt_le_dec 0 q0). 2:{ lra. }
+      tauto.
+Qed.
 
 Theorem hoare_store_sound : forall P e1 e2 p v,
   derives P (andp (eqp e1 p) (eqp e2 v)) ->
-  valid (sepcon P (mapsto_ p)) (CStore e1 e2) (sepcon P (mapsto p v)) falsep falsep.
+  valid (sepcon P (fullper p)) (CStore e1 e2) (sepcon P (mapsto p v)) falsep falsep.
 Proof.
-  unfold derives, valid; intros.
-  split. unfold sepcon, SepCon in *.
-  destruct H0 as [st11 [st12 [? [? ?]]]].
+  unfold derives, valid. intros.
+  unfold andp in H.
+  ufSepcon H0. destruct H0 as [st11 [st12 [? [? ?]]]].
+  split.
   { unfold not; intros.
-    simpl in H1.
-    specialize (H st11 H0).
-    unfold andp, eqp in H.
+    simpl in H3.
+    pose proof H st11 H0.
+    unfold eqp in H4. destruct H4.
+    pose proof (andjoin1 e1 p st11 st12 st1 H4 H2).
+    rewrite H6 in H3.
+    pose proof (andjoin1 e2 v st11 st12 st1 H5 H2).
+    rewrite H7 in H3.
+    assert (exists x, snd st1 p = Some x).
+    { ufStatej H2. destruct H2.
+      ufHeapj H8. specialize (H8 p). rewrite ufoptionj in H8.
+      unfold fullper in H1. destruct H1.
+      destruct H1 as [z ?].
+      destruct H8 as [? | [? | [? | ?]]].
+      + destruct H8 as [? [? ?]]. rewrite H10 in H1. inversion H1.
+      + destruct H8 as [x [? [? ?]]]. exists x; tauto.
+      + destruct H8 as [x [? [? ?]]]. rewrite H10 in H1; inversion H1.
+      + destruct H8 as [x1 [x2 [x [? [? [? ?]]]]]].
+        exists x; tauto. }
+    destruct H8 as [x ?].
+    rewrite H8 in H3.
+    unfold fullper in H1. destruct H1 as [[z ?] ?].
+    assert (snd st1 p = Some (inl (1%Q, z))).
+    { ufStatej H2. destruct H2.
+      ufHeapj H10. specialize (H10 p). rewrite ufoptionj in H10.
+      destruct H10 as [? | [? | [? | ?]]].
+      + destruct H10 as [? [? ?]]. rewrite H11 in H1. inversion H1.
+      + destruct H10 as [x' [? [? ?]]]. rewrite H11 in H1. inversion H1. 
+        rewrite H1 in H12. tauto.
+      + destruct H10 as [x' [? [? ?]]]. rewrite H11 in H1. inversion H1.
+      + destruct H10 as [x1 [x2 [x' [? [? [? ?]]]]]].
+        unfold QZandLock_Join in H13. rewrite ufsumj in H13.
+        destruct H13. 2:{
+        destruct H13 as [xr1 [xr2 [xr [? [? [? ?]]]]]].
+        rewrite H11 in H1. rewrite H14 in H1. inversion H1. }
+        destruct H13 as [xl1 [xl2 [xl [? [? [? ?]]]]]].
+        rewrite H11 in H1. rewrite H14 in H1. inversion H1.
+        unfold QZ_Join in H16. 
+        unfold OSAGenerators.prod_Join in H16.
+        destruct H16.
+        unfold SeparationAlgebra.join in H16, H17.
+        unfold Q_Join in H16. unfold Z_Join in H17.
+        unfold OSAGenerators.equiv_Join in H17.
+        destruct H17.
+        destruct xl as (q', z'). simpl in H16, H17, H19.
+        rewrite H18 in H19. simpl in H19. subst z'.
+        rewrite <-H19 in H15.
+        rewrite H18 in H16. simpl in H16.
+        assert (q' == 1). {lra. }
+        rewrite H12. rewrite H15. lra. }
+    rewrite H8 in H10. inversion H10.
+    rewrite H12 in H3. lra. }
+  split.
+  { intros. 
+    pose proof (H st11 H0).
+    unfold eqp in H4; destruct H4.
+    assert (aeval e1 st1 = Some p).
+    { eapply andjoin1; [exact H4 | exact H2]. }
+    assert (aeval e2 st1 = Some v).
+    { eapply andjoin1; [exact H5 | exact H2]. }
+    ufsepcon. 
+    remember (fst st12, heap_update (snd st12) p (Some v)) as st22.
+    exists st11, st22.
+    split; try tauto. split.
+    { unfold mapsto. unfold fullper in H1.
+      destruct H1 as [[v' ?] ?].
+      split.
+      + subst st22. unfold snd at 1.
+        unfold heap_update. destruct (Z.eq_dec p p); try tauto.
+        exists 1%Q. rewrite H1. tauto.
+      + subst st22. intros.
+        unfold snd at 1. unfold heap_update.
+        destruct (Z.eq_dec p' p); try tauto.
+        exact (H8 p' n). }
+    simpl in H3; rewrite H6, H7 in H3.
+    remember (snd st1 p) as s'.
+    destruct (s'); try tauto.
+    destruct s; try tauto.
+    destruct p0 as (q1, z1).
+    remember (snd st2 p) as s''.
+    destruct s''; try tauto.
+    destruct s; try tauto.
+    destruct p0 as (q2, z2).
+    destruct H3 as [? [? [? [? ?]]]].
+    ufstatej. ufStatej H2.
+    unfold SeparationAlgebra.join in H2.
+    destruct H2.
+    split.
+    { subst st22. unfold fst at 2. rewrite <-H11. tauto. }
+    ufheapj. ufHeapj H12.
+    intros pp. specialize (H12 pp).
+    rewrite ufoptionj in *. destruct H12 as [? | [? | [? | ?]]].
+    + left. split; try tauto. destruct H12 as [? [? ?]].
+      subst st22. unfold heap_update.  unfold snd at 1.
+      destruct (Z.eq_dec pp p).
+      - subst pp. rewrite H14 in Heqs'. inversion Heqs'.
+      - specialize (H10 pp n). rewrite H10. tauto.
+    + right; left.  destruct H12 as [vv [? [? ?]]].
+      subst st22. unfold snd at 2. unfold heap_update.
+      destruct (Z.eq_dec pp p).
+      - subst pp.
+        unfold fullper in H1. destruct H1.
+        destruct H1 as [v' ?].
+        rewrite H1. exists (inl (1%Q, v)).
+        split; try split; try tauto.
+        rewrite <-Heqs''. rewrite H9. 
+        rewrite H8. tauto.
+      - exists vv.
+        specialize (H10 pp n). rewrite H10. tauto.
+    + right; right; left. destruct H12 as [vv [? [? ?]]].
+      subst st22. unfold snd at 2. unfold heap_update.
+      destruct (Z.eq_dec pp p).
+      - subst pp.
+        unfold fullper in H1. destruct H1 as [[v' ?] ?].
+        rewrite H13 in H1. inversion H1.
+      - exists vv.
+        specialize (H10 pp n). rewrite H10. tauto.
+    + right; right; right. 
+      destruct H12 as [vv1 [vv2 [vv [? [? [? ?]]]]]].
+      subst st22. unfold heap_update.
+      unfold snd at 2. destruct (Z.eq_dec pp p).
+      - subst pp. rewrite H13.
+        unfold QZandLock_Join in *. rewrite ufsumj in H15.
+        destruct H15.
+        2:{ destruct H15 as [? [? [? [? [? [? ?]]]]]]. 
+            rewrite H17 in H14. rewrite H14 in Heqs'. inversion Heqs'. }
+        destruct H15 as [vl1 [vl2 [vl [? [? [? ?]]]]]].
+        subst vv1 vv2 vv. 
+        destruct vl1 as (qq1, qz1).
+        destruct vl2 as (qq2, qz2).
+        rewrite H14 in Heqs'. inversion Heqs'. subst vl.
+        subst. clear Heqs'.
+        exists (inl (qq1, z1)), (inl (qq2, z1)), (inl (1%Q, z1)).
+        unfold QZ_Join in H18. unfold OSAGenerators.prod_Join in H18.
+        unfold SeparationAlgebra.join in H18.
+        destruct H18. unfold Z_Join in H8. unfold OSAGenerators.equiv_Join in H8.
+        destruct H8. inversion H8. inversion H9. unfold snd in H15, H16. subst.
+        split.
+        { rewrite H12. tauto. }
+        split.
+        { rewrite H} 
 
 
+
+        repeat eexists. exact H12. rewrite Heqs''. tauto.
+        rewrite ufsumj. left.
+        eexists. eexists. eexists.
+        split; [tauto |]. split; [tauto |]. split; [tauto |].
+        unfold QZ_Join in *. unfold OSAGenerators.prod_Join in *.
+        unfold fst, snd in H18. unfold SeparationAlgebra.join in H18.
+        split. 2:{
+        unfold SeparationAlgebra.join, snd.
+        unfold Z_Join. unfold OSAGenerators.equiv_Join.
+        destruct H18. unfold Z_Join in H16. unfold OSAGenerators.equiv_Join in H16.
+        subst. split; try tauto.
+
+          
+
+
+    
+
+
+
+
+
+      
 
